theories/lang/lang_extra.v
@@ -10,7 +10,7 @@ Context `{HyperConst : !HypervisorConstants}.
 Context `{HyperParams : !HypervisorParameters}.
 
 Lemma check_access_page_mem_eq {σ i a} :
-  check_access_page' σ i (to_pid_aligned a) =
+  check_access_page σ i (to_pid_aligned a) =
   check_access_addr σ i a.
 Proof.
   rewrite /check_access_addr; done.
