theories/lang/pagetable_extra.v
@@ -184,921 +184,948 @@ Proof.
   rewrite IHps //.
 Qed.
 
-(* TODO: update_access_batch_preserve_mb (easy) *)
-(* TODO: update_ownership_batch_preserve_mb (hard) *)
-(* TODO: *)
-
-Lemma get_pagetable_gmap_checkb {σ} p v s:
- (get_pagetable_gmap σ) !! p = Some (v, s)->
- (p ∈ s <->
-  ∃ perm, (proj (get_vm_page_table σ i)) !! p =Some perm ∧ checkb perm = true).
+Lemma update_access_batch_preserve_mb σ ps:
+ (get_mb_gmap (update_access_batch σ ps)) = (get_mb_gmap σ).
 Proof.
-  intros.
-  rewrite /get_access_gmap in H.
-  apply (elem_of_list_to_map_2 _ i s) in H.
-  inv_map_in. clear H0.
-  inversion H.
-  subst.
-  clear H.
-  split.
-  - intro H. apply elem_of_list_to_set in H.
-    inv_map_in.
-    apply elem_of_list_In in H0.
-    apply elem_of_map_to_list' in H0.
-    apply map_filter_lookup_Some in H0.
-    destruct H0.
-    exists x.2.
-    split;eauto.
-      by subst p.
-  - intros H.
-    destruct H.
-    apply elem_of_list_to_set.
-    apply elem_of_list_In.
-    apply in_map_iff.
-    exists (p,x).
-    split;eauto.
-    apply elem_of_list_In.
-    apply elem_of_map_to_list'.
-    apply map_filter_lookup_Some.
-    done.
+  rewrite /get_mb_gmap /update_access_batch /update_access_global_batch /=.
+  f_equal.
+ Qed.
+
+Lemma update_ownership_batch_preserve_mb σ ps:
+ (get_mb_gmap (update_ownership_batch σ ps)) = (get_mb_gmap σ).
+Proof.
+  rewrite /get_mb_gmap /=.
+  f_equal.
 Qed.
 
-Lemma get_owned_gmap_is_owned {σ i sown} p:
- (get_owned_gmap σ) !! i = Some sown->
- (p ∈ sown <->
-  ∃ perm, (get_vm_page_table σ i).1 !! p =Some perm ∧ is_owned perm = true).
+(* TODO: *)
+
+(* Lemma get_pagetable_gmap_checkb {σ} p v s: *)
+(*  (get_pagetable_gmap σ) !! p = Some (v, s)-> *)
+(*  (p ∈ s <-> *)
+(*   ∃ perm, (proj (get_vm_page_table σ i)) !! p =Some perm ∧ checkb perm = true). *)
+(* Proof. *)
+(*   intros. *)
+(*   rewrite /get_access_gmap in H. *)
+(*   apply (elem_of_list_to_map_2 _ i s) in H. *)
+(*   inv_map_in. clear H0. *)
+(*   inversion H. *)
+(*   subst. *)
+(*   clear H. *)
+(*   split. *)
+(*   - intro H. apply elem_of_list_to_set in H. *)
+(*     inv_map_in. *)
+(*     apply elem_of_list_In in H0. *)
+(*     apply elem_of_map_to_list' in H0. *)
+(*     apply map_filter_lookup_Some in H0. *)
+(*     destruct H0. *)
+(*     exists x.2. *)
+(*     split;eauto. *)
+(*       by subst p. *)
+(*   - intros H. *)
+(*     destruct H. *)
+(*     apply elem_of_list_to_set. *)
+(*     apply elem_of_list_In. *)
+(*     apply in_map_iff. *)
+(*     exists (p,x). *)
+(*     split;eauto. *)
+(*     apply elem_of_list_In. *)
+(*     apply elem_of_map_to_list'. *)
+(*     apply map_filter_lookup_Some. *)
+(*     done. *)
+(* Qed. *)
+
+(*--- prove having mappings in gmap implies owership/access to pages in opsem ---*)
+
+Lemma get_owned_gmap_is_owned {σ} p i:
+ (get_owned_gmap σ) !! p = Some (i,Owned) ->
+ ∃ acc, (get_page_table σ) !! p =Some (i,acc).
 Proof.
   intros.
   rewrite /get_owned_gmap in H.
-    by apply get_pagetable_gmap_checkb.
+  apply (elem_of_list_to_map_2 _ p (i,Owned) ) in H.
+  (* inv_map_in. clear H0. *)
+    apply elem_of_map_to_list' in H.
+  simpl in H.
+  rewrite lookup_fmap in H.
+  destruct (get_page_table σ !! p) eqn:Heqn.
+  exists p0.2.
+  rewrite Heqn /= in H.
+  inversion H.
+  destruct p0;done.
+  rewrite Heqn in H.
+  done.
 Qed.
 
-Lemma get_access_gmap_is_accessible {σ i sacc} p:
- (get_access_gmap σ) !! i = Some  sacc->
- (p ∈ sacc <->
-  ∃ perm, (get_vm_page_table σ i).2 !! p =Some perm ∧ is_accessible perm = true).
+Lemma get_access_gmap_is_accessible {σ} p sacc:
+ (get_access_gmap σ) !! p = Some (1%Qp, GSet sacc) ->
+  ∃ v, (get_page_table σ) !! p = Some (v,sacc).
 Proof.
   intros.
   rewrite /get_access_gmap in H.
-    by apply get_pagetable_gmap_checkb.
+  (* apply (elem_of_list_to_map_2 _ p (1%Qp,GSet sacc) ) in H. *)
+  (* inv_map_in. clear H0. *)
+    (* apply elem_of_map_to_list' in H. *)
+  (* simpl in H. *)
+  rewrite lookup_fmap in H.
+  destruct (get_page_table σ !! p) eqn:Heqn.
+  exists p0.1.
+  rewrite Heqn /= in H.
+  inversion H.
+  destruct p0;done.
+  rewrite Heqn in H.
+  done.
 Qed.
 
-Lemma get_excl_gmap_is_exclusive_true {σ i sexcl} p:
- (get_excl_gmap σ) !! i = Some  sexcl->
- (p ∈ sexcl<->
-  ∃ perm, (get_vm_page_table σ i).2 !! p =Some perm ∧ is_exclusive perm = true).
-Proof.
-  intros.
-  rewrite /get_excl_gmap in H.
-    by apply get_pagetable_gmap_checkb.
-Qed.
+(* Lemma get_access_gmap_is_exclusive {σ} p i : *)
+(*  (get_access_gmap σ) !! p = Some  (1%Qp, GSet {[i]}) -> *)
+(*   ∃ v , (get_page_table σ) !! p =Some(v, {[i]}) . *)
 
-Lemma update_access_batch_update_pagetable_diff {σ i s p} {sps:gset PID}
-      (checkb: access->bool) (ps: list PID):
- sps = (list_to_set ps)->
- i = (get_current_vm σ) ->
- checkb p = false ->
- (get_pagetable_gmap σ (λ pt,pt.2) checkb) !! i = Some s ->
- (get_pagetable_gmap (update_access_batch σ ps p)  (λ pt,pt.2) checkb) =
- <[(get_current_vm σ):= s ∖ sps]>(get_pagetable_gmap σ (λ pt,pt.2) checkb).
-Proof.
-  intros Hsps Hi Hcheckb Hlookup.
-  rewrite /get_pagetable_gmap.
-  apply (@map_eq VMID (gmap VMID) _ _ _ _ _ _ _ _ gmap_finmap);eauto.
-  intro.
-  rewrite -Hi.
-  destruct(decide (i0 = i)).
-  - subst i0. rewrite lookup_insert.
-    assert(Hgoal : list_to_set
-                     (map (λ p : PID * access, p.1)
-                          (map_to_list (filter (λ p : PID * access, checkb p.2 = true)
-                                               (get_vm_page_table (update_access_batch σ ps p) i).2))) = s ∖ sps).
-    { apply set_eq.
-      intro.
-      rewrite elem_of_list_to_set.
-      split.
-      * intros.
-        inv_map_in.
-        apply elem_of_list_In in H0.
-        apply (elem_of_map_to_list' _ x0) in H0.
-        apply map_filter_lookup_Some in H0.
-        destruct H0 as [Hlookup' Hcheckbtrue].
-        simplify_eq /=.
-        rewrite /get_vm_page_table /get_page_tables /update_access_batch
-                /update_access_global_batch //= in Hlookup'.
-        rewrite vlookup_insert in Hlookup'.
-        apply elem_of_difference.
-        induction ps; simpl in *.
-        -- split;[|set_solver].
-           apply ((get_pagetable_gmap_checkb (λ pt,pt.2) checkb) x0.1 Hlookup).
-           exists (x0.2).
-           split;eauto.
-        -- assert (Hneq: a ≠ x0.1).
-           { destruct (decide (a=x0.1));eauto.
-             subst a.
-             rewrite lookup_insert in Hlookup'.
-             inversion Hlookup'.
-             rewrite -H0  Hcheckb // in Hcheckbtrue.
-           }
-           rewrite not_elem_of_union.
-           assert (Himp : x0.1 ∈ s ∧ x0.1 ∉ ((list_to_set ps):gset PID)
-                          ->(x0.1 ∈ s ∧ (x0.1 ∉ ({[a]}:gset PID)) ∧ x0.1 ∉ ((list_to_set ps):gset PID))).
-           { intros. destruct H; split;eauto. split. set_solver. done. }
-           apply Himp.
-           apply IHps;eauto.
-           rewrite lookup_insert_ne in Hlookup';done.
-      * intros Hin.
-        apply elem_of_difference in Hin.
-        destruct Hin as [Hin Hnotin].
-        apply ((get_pagetable_gmap_checkb (λ pt,pt.2) checkb) x Hlookup) in Hin;eauto.
-        destruct Hin.
-        destruct H.
-        inv_map_in.
-        exists (x,x0).
-        split;eauto.
-        apply elem_of_list_In .
-        apply  elem_of_map_to_list.
-        apply map_filter_lookup_Some.
-        rewrite /get_vm_page_table /get_page_tables /update_access_batch
-                /update_access_global_batch /=.
-        rewrite -Hi vlookup_insert.
-        split;eauto.
-        generalize dependent sps.
-        induction ps;simpl.
-        done.
-        intros.
-        assert (Hneq: a ≠ x).
-        { set_solver. }
-        rewrite lookup_insert_ne;eauto.
-        apply (IHps (list_to_set ps));eauto.
-        set_solver.
-    }
-    apply (@elem_of_list_to_map_1' VMID (gmap VMID) _ _ _ _ _ _ _ _ gmap_finmap).
-    + intros.
-      inv_map_in.
-      inversion H.
-      do 3 f_equal.
-      clear H3 H0 H.
-      subst x.
-      symmetry.
-      apply Hgoal.
-    + inv_map_in.
-      exists i.
-      split;[|apply in_list_of_vmids].
-      do 4 f_equal.
-      apply Hgoal.
-  - rewrite (lookup_insert_ne _ i i0 _);eauto.
-    set (l:= (map (λ v,  (v, get_pagetable_gset (update_access_batch σ ps p) v (λ pt : page_table, pt.2) checkb)) list_of_vmids)) in *.
-    destruct (list_to_map l !! i0) eqn:Heqn.
-    + apply (elem_of_list_to_map_2 l i0 g) in Heqn.
-      apply elem_of_list_In in Heqn.
-      apply in_map_iff in Heqn.
-      inversion Heqn;clear Heqn.
-      destruct H as [H HIn];inversion H;subst;clear H.
-      symmetry.
-      eapply elem_of_list_to_map_1'.
-      * intros.
-        inv_map_in.
-        inversion H.
-        rewrite /get_pagetable_gset.
-        do 4 f_equal.
-        rewrite /get_vm_page_table update_access_batch_preserve_other_page_tables //.
-      * inv_map_in.
-        exists i0.
-        split;eauto.
-        rewrite /get_pagetable_gset.
-        do 6 f_equal.
-        rewrite /get_vm_page_table update_access_batch_preserve_other_page_tables //.
-    + apply (@not_elem_of_list_to_map_2 VMID (gmap VMID) _ _ _ _ _ _ _ _ gmap_finmap) in Heqn.
-      symmetry.
-      apply not_elem_of_list_to_map_1.
-      intro P.
-      apply Heqn.
-      apply elem_of_list_In.
-      apply in_map_iff.
-      apply elem_of_list_In in P.
-      apply in_map_iff in P.
-      destruct P.
-      exists x.
-      destruct H.
-      split;eauto.
-      apply in_map_iff.
-      apply in_map_iff in H0.
-      destruct H0.
-      exists x0.
-      destruct H0.
-      split;eauto.
-      rewrite -H0 /get_pagetable_gset.
-      do 6 f_equal.
-      rewrite /get_vm_page_table update_access_batch_preserve_other_page_tables //.
-      destruct x.
-      inversion H0.
-        by subst.
-Qed.
+(* XXX what should the following lemma look like? *)
+(* Lemma update_access_batch_update_access_gmap {σ i s p} {sps:gset PID} *)
+(*       (ps: list PID): *)
+(*  sps = (list_to_set ps) -> *)
+(*  i = (get_current_vm σ) -> *)
+(*  (∀ p, p ∈ ps -> ∃ q sacc, (get_access_gmap σ) !! p = Some (q, sacc) -> *)
+(*                           (get_access_gmap (update_access_batch σ ps)) !! p = Some (q,sacc ∪ {[i]})). *)
+(* Proof. *)
+(*   intros Hsps Hi Hcheckb Hlookup. *)
+(*   rewrite /get_pagetable_gmap. *)
+(*   apply (@map_eq VMID (gmap VMID) _ _ _ _ _ _ _ _ gmap_finmap);eauto. *)
+(*   intro. *)
+(*   rewrite -Hi. *)
+(*   destruct(decide (i0 = i)). *)
+(*   - subst i0. rewrite lookup_insert. *)
+(*     assert(Hgoal : list_to_set *)
+(*                      (map (λ p : PID * access, p.1) *)
+(*                           (map_to_list (filter (λ p : PID * access, checkb p.2 = true) *)
+(*                                                (get_vm_page_table (update_access_batch σ ps p) i).2))) = s ∖ sps). *)
+(*     { apply set_eq. *)
+(*       intro. *)
+(*       rewrite elem_of_list_to_set. *)
+(*       split. *)
+(*       * intros. *)
+(*         inv_map_in. *)
+(*         apply elem_of_list_In in H0. *)
+(*         apply (elem_of_map_to_list' _ x0) in H0. *)
+(*         apply map_filter_lookup_Some in H0. *)
+(*         destruct H0 as [Hlookup' Hcheckbtrue]. *)
+(*         simplify_eq /=. *)
+(*         rewrite /get_vm_page_table /get_page_tables /update_access_batch *)
+(*                 /update_access_global_batch //= in Hlookup'. *)
+(*         rewrite vlookup_insert in Hlookup'. *)
+(*         apply elem_of_difference. *)
+(*         induction ps; simpl in *. *)
+(*         -- split;[|set_solver]. *)
+(*            apply ((get_pagetable_gmap_checkb (λ pt,pt.2) checkb) x0.1 Hlookup). *)
+(*            exists (x0.2). *)
+(*            split;eauto. *)
+(*         -- assert (Hneq: a ≠ x0.1). *)
+(*            { destruct (decide (a=x0.1));eauto. *)
+(*              subst a. *)
+(*              rewrite lookup_insert in Hlookup'. *)
+(*              inversion Hlookup'. *)
+(*              rewrite -H0  Hcheckb // in Hcheckbtrue. *)
+(*            } *)
+(*            rewrite not_elem_of_union. *)
+(*            assert (Himp : x0.1 ∈ s ∧ x0.1 ∉ ((list_to_set ps):gset PID) *)
+(*                           ->(x0.1 ∈ s ∧ (x0.1 ∉ ({[a]}:gset PID)) ∧ x0.1 ∉ ((list_to_set ps):gset PID))). *)
+(*            { intros. destruct H; split;eauto. split. set_solver. done. } *)
+(*            apply Himp. *)
+(*            apply IHps;eauto. *)
+(*            rewrite lookup_insert_ne in Hlookup';done. *)
+(*       * intros Hin. *)
+(*         apply elem_of_difference in Hin. *)
+(*         destruct Hin as [Hin Hnotin]. *)
+(*         apply ((get_pagetable_gmap_checkb (λ pt,pt.2) checkb) x Hlookup) in Hin;eauto. *)
+(*         destruct Hin. *)
+(*         destruct H. *)
+(*         inv_map_in. *)
+(*         exists (x,x0). *)
+(*         split;eauto. *)
+(*         apply elem_of_list_In . *)
+(*         apply  elem_of_map_to_list. *)
+(*         apply map_filter_lookup_Some. *)
+(*         rewrite /get_vm_page_table /get_page_tables /update_access_batch *)
+(*                 /update_access_global_batch /=. *)
+(*         rewrite -Hi vlookup_insert. *)
+(*         split;eauto. *)
+(*         generalize dependent sps. *)
+(*         induction ps;simpl. *)
+(*         done. *)
+(*         intros. *)
+(*         assert (Hneq: a ≠ x). *)
+(*         { set_solver. } *)
+(*         rewrite lookup_insert_ne;eauto. *)
+(*         apply (IHps (list_to_set ps));eauto. *)
+(*         set_solver. *)
+(*     } *)
+(*     apply (@elem_of_list_to_map_1' VMID (gmap VMID) _ _ _ _ _ _ _ _ gmap_finmap). *)
+(*     + intros. *)
+(*       inv_map_in. *)
+(*       inversion H. *)
+(*       do 3 f_equal. *)
+(*       clear H3 H0 H. *)
+(*       subst x. *)
+(*       symmetry. *)
+(*       apply Hgoal. *)
+(*     + inv_map_in. *)
+(*       exists i. *)
+(*       split;[|apply in_list_of_vmids]. *)
+(*       do 4 f_equal. *)
+(*       apply Hgoal. *)
+(*   - rewrite (lookup_insert_ne _ i i0 _);eauto. *)
+(*     set (l:= (map (λ v,  (v, get_pagetable_gset (update_access_batch σ ps p) v (λ pt : page_table, pt.2) checkb)) list_of_vmids)) in *. *)
+(*     destruct (list_to_map l !! i0) eqn:Heqn. *)
+(*     + apply (elem_of_list_to_map_2 l i0 g) in Heqn. *)
+(*       apply elem_of_list_In in Heqn. *)
+(*       apply in_map_iff in Heqn. *)
+(*       inversion Heqn;clear Heqn. *)
+(*       destruct H as [H HIn];inversion H;subst;clear H. *)
+(*       symmetry. *)
+(*       eapply elem_of_list_to_map_1'. *)
+(*       * intros. *)
+(*         inv_map_in. *)
+(*         inversion H. *)
+(*         rewrite /get_pagetable_gset. *)
+(*         do 4 f_equal. *)
+(*         rewrite /get_vm_page_table update_access_batch_preserve_other_page_tables //. *)
+(*       * inv_map_in. *)
+(*         exists i0. *)
+(*         split;eauto. *)
+(*         rewrite /get_pagetable_gset. *)
+(*         do 6 f_equal. *)
+(*         rewrite /get_vm_page_table update_access_batch_preserve_other_page_tables //. *)
+(*     + apply (@not_elem_of_list_to_map_2 VMID (gmap VMID) _ _ _ _ _ _ _ _ gmap_finmap) in Heqn. *)
+(*       symmetry. *)
+(*       apply not_elem_of_list_to_map_1. *)
+(*       intro P. *)
+(*       apply Heqn. *)
+(*       apply elem_of_list_In. *)
+(*       apply in_map_iff. *)
+(*       apply elem_of_list_In in P. *)
+(*       apply in_map_iff in P. *)
+(*       destruct P. *)
+(*       exists x. *)
+(*       destruct H. *)
+(*       split;eauto. *)
+(*       apply in_map_iff. *)
+(*       apply in_map_iff in H0. *)
+(*       destruct H0. *)
+(*       exists x0. *)
+(*       destruct H0. *)
+(*       split;eauto. *)
+(*       rewrite -H0 /get_pagetable_gset. *)
+(*       do 6 f_equal. *)
+(*       rewrite /get_vm_page_table update_access_batch_preserve_other_page_tables //. *)
+(*       destruct x. *)
+(*       inversion H0. *)
+(*         by subst. *)
+(* Qed. *)
 
-Lemma update_access_batch_update_access_diff{σ i sacc} {sps:gset PID} (ps: list PID):
- sps = (list_to_set ps)->
- i = (get_current_vm σ) ->
- (get_access_gmap σ) !! i = Some sacc ->
- get_access_gmap (update_access_batch σ ps NoAccess) =
- <[(get_current_vm σ):= (sacc∖ sps)]>(get_access_gmap σ).
-Proof.
-  intros.
-  apply (@update_access_batch_update_pagetable_diff _ i);eauto.
-Qed.
+(* Lemma update_access_batch_update_access_diff{σ i sacc} {sps:gset PID} (ps: list PID): *)
+(*  sps = (list_to_set ps)-> *)
+(*  i = (get_current_vm σ) -> *)
+(*  (get_access_gmap σ) !! i = Some sacc -> *)
+(*  get_access_gmap (update_access_batch σ ps NoAccess) = *)
+(*  <[(get_current_vm σ):= (sacc∖ sps)]>(get_access_gmap σ). *)
+(* Proof. *)
+(*   intros. *)
+(*   apply (@update_access_batch_update_pagetable_diff _ i);eauto. *)
+(* Qed. *)
 
-Lemma update_access_batch_update_excl_diff{σ i sexcl p} {sps:gset PID} (ps: list PID):
- sps = (list_to_set ps)->
- i = (get_current_vm σ) ->
- is_exclusive p = false ->                                              
- (get_excl_gmap σ) !! i = Some sexcl ->
- get_excl_gmap (update_access_batch σ ps p) =
- <[(get_current_vm σ):= (sexcl ∖ sps)]>(get_excl_gmap σ).
-Proof.
-  intros.
-  apply (@update_access_batch_update_pagetable_diff _ i);eauto.
-Qed.
+(* Lemma update_access_batch_update_excl_diff{σ i sexcl p} {sps:gset PID} (ps: list PID): *)
+(*  sps = (list_to_set ps)-> *)
+(*  i = (get_current_vm σ) -> *)
+(*  is_exclusive p = false ->                                               *)
+(*  (get_excl_gmap σ) !! i = Some sexcl -> *)
+(*  get_excl_gmap (update_access_batch σ ps p) = *)
+(*  <[(get_current_vm σ):= (sexcl ∖ sps)]>(get_excl_gmap σ). *)
+(* Proof. *)
+(*   intros. *)
+(*   apply (@update_access_batch_update_pagetable_diff _ i);eauto. *)
+(* Qed. *)
 
-Lemma update_ownership_batch_update_pagetable_union {σ i sown} {sps:gset PID} (ps: list PID):
- sps = (list_to_set ps)->
- i = (get_current_vm σ)->
- (get_owned_gmap σ) !! i = Some sown ->
- get_owned_gmap (update_ownership_batch σ ps Owned) =
- <[i:= sown ∪ sps]>(get_owned_gmap σ).
-Proof.
-  intros.
-  rewrite /get_owned_gmap /get_pagetable_gmap.
-  apply (@map_eq VMID (gmap VMID) _ _ _ _ _ _ _ _ gmap_finmap);eauto.
-  intro.
-  destruct(decide (i0 = i)).
-  - subst i0. rewrite lookup_insert.
-    assert(Hgoal: get_pagetable_gset (update_ownership_batch σ ps Owned) i (λ pt : page_table, pt.1) is_owned
-                  = sown ∪ sps).
-    {
-      apply set_eq.
-      intro.
-      rewrite elem_of_list_to_set.
-      split.
-      * intros.
-        inv_map_in.
-        apply elem_of_list_In in H3.
-        apply (elem_of_map_to_list' _ x0) in H3.
-        apply map_filter_lookup_Some in H3.
-        destruct H3.
-        simplify_eq /=.
-        rewrite /get_vm_page_table /get_page_tables /update_ownership_batch
-                /update_ownership_global_batch //= in H3.
-        rewrite vlookup_insert in H3.
-        apply elem_of_union.
-        induction ps; simpl in *.
-        -- left.
-           apply (get_owned_gmap_is_owned x0.1 H1).
-           exists (x0.2).
-           split;eauto.
-        -- destruct (decide (a=x0.1)).
-           right;set_solver.
-           assert (Himp :(x0.1 ∈ sown ∨ x0.1 ∈ ((list_to_set ps):gset PID))
-                         ->(x0.1 ∈ sown ∨ x0.1 ∈ {[a]} ∪ ((list_to_set ps):gset PID))).
-           { intros. destruct H. left;done. right; set_solver. }
-           apply Himp.
-           apply IHps;eauto.
-           rewrite lookup_insert_ne in H3;done.
-      * intros.
-        apply elem_of_union in H2.
-        destruct H2.
-        apply (get_owned_gmap_is_owned x H1) in H2;eauto.
-        destruct H2.
-        destruct H2.
-        inv_map_in.
-        exists (x,x0).
-        split;eauto.
-        apply elem_of_list_In .
-        apply elem_of_map_to_list.
-        apply map_filter_lookup_Some.
-        rewrite /get_vm_page_table /get_page_tables /update_ownership_batch
-                /update_ownership_global_batch /=.
-        rewrite -H0 vlookup_insert.
-        destruct H1;split;eauto.
-        generalize dependent sps.
-        induction ps;simpl in *.
-        done.
-        intros.
-        destruct (decide (x=a)).
-        subst a.
-        rewrite lookup_insert.
-        rewrite /is_owned in H3.
-        destruct x0;eauto.
-        done.
-        rewrite lookup_insert_ne;eauto.
-        inv_map_in.
-        exists (x,Owned).
-        split;eauto.
-        apply elem_of_list_In .
-        apply elem_of_map_to_list.
-        apply map_filter_lookup_Some.
-        rewrite /get_vm_page_table /get_page_tables /update_ownership_batch
-                /update_ownership_global_batch /=.
-        split;eauto.
-        rewrite -H0 vlookup_insert //=.
-        generalize dependent sps.
-        induction ps;simpl in *.
-        intros.
-        set_solver.
-        intros.
-        destruct (decide (x=a)).
-        subst a.
-        rewrite lookup_insert //.
-        rewrite lookup_insert_ne;eauto.
-        apply (IHps (list_to_set ps));eauto.
-        set_solver.
-    }
-    apply (@elem_of_list_to_map_1' VMID (gmap VMID) _ _ _ _ _ _ _ _ gmap_finmap).
-    + intros.
-      inv_map_in.
-      inversion H2.
-      do 3 f_equal.
-      clear H6 H3 H2.
-      subst x.
-      symmetry.
-      apply Hgoal.
-    + inv_map_in.
-      exists i.
-      split;[|apply in_list_of_vmids].
-      do 4 f_equal.
-      apply Hgoal.
-  - rewrite (lookup_insert_ne _ i i0 _);eauto.
-    set (l:= (map
-                (λ v,
-                 (v, get_pagetable_gset (update_ownership_batch σ ps Owned) v (λ pt : page_table, pt.1) is_owned))
-                list_of_vmids)) in *.
-    destruct (list_to_map l !! i0) eqn:Heqn.
-    + apply (elem_of_list_to_map_2 l i0 g) in Heqn.
-      apply elem_of_list_In in Heqn.
-      apply in_map_iff in Heqn.
-      inversion Heqn;clear Heqn.
-      destruct H2 as [H3 HIn];inversion H3;subst;clear H3.
-      symmetry.
-      apply elem_of_list_to_map_1'.
-      *  intros.
-         inv_map_in.
-         inversion H.
-         rewrite /get_pagetable_gset.
-         do 5 f_equal.
-         rewrite /get_vm_page_table update_ownership_batch_preserve_other_page_tables //.
-      * inv_map_in.
-        exists i0.
-        split;eauto.
-        rewrite /get_pagetable_gset.
-        do 6 f_equal.
-        rewrite /get_vm_page_table update_ownership_batch_preserve_other_page_tables //.
-    + apply (@not_elem_of_list_to_map_2 VMID (gmap VMID) _ _ _ _ _ _ _ _ gmap_finmap) in Heqn.
-      symmetry.
-      apply not_elem_of_list_to_map_1.
-      intro P.
-      apply Heqn.
-      apply elem_of_list_In.
-      apply in_map_iff.
-      apply elem_of_list_In in P.
-      apply in_map_iff in P.
-      destruct P.
-      exists x.
-      destruct H2.
-      split;eauto.
-      apply in_map_iff.
-      apply in_map_iff in H3.
-      destruct H3.
-      exists x0.
-      destruct H3.
-      split;eauto.
-      rewrite -H3 /get_pagetable_gset.
-      do 6 f_equal.
-      rewrite /get_vm_page_table update_ownership_batch_preserve_other_page_tables //.
-      destruct x.
-      simpl in H2;inversion H3.
-        by subst.
-Qed.
+(* Lemma update_ownership_batch_update_pagetable_union {σ i sown} {sps:gset PID} (ps: list PID): *)
+(*  sps = (list_to_set ps)-> *)
+(*  i = (get_current_vm σ)-> *)
+(*  (get_owned_gmap σ) !! i = Some sown -> *)
+(*  get_owned_gmap (update_ownership_batch σ ps Owned) = *)
+(*  <[i:= sown ∪ sps]>(get_owned_gmap σ). *)
+(* Proof. *)
+(*   intros. *)
+(*   rewrite /get_owned_gmap /get_pagetable_gmap. *)
+(*   apply (@map_eq VMID (gmap VMID) _ _ _ _ _ _ _ _ gmap_finmap);eauto. *)
+(*   intro. *)
+(*   destruct(decide (i0 = i)). *)
+(*   - subst i0. rewrite lookup_insert. *)
+(*     assert(Hgoal: get_pagetable_gset (update_ownership_batch σ ps Owned) i (λ pt : page_table, pt.1) is_owned *)
+(*                   = sown ∪ sps). *)
+(*     { *)
+(*       apply set_eq. *)
+(*       intro. *)
+(*       rewrite elem_of_list_to_set. *)
+(*       split. *)
+(*       * intros. *)
+(*         inv_map_in. *)
+(*         apply elem_of_list_In in H3. *)
+(*         apply (elem_of_map_to_list' _ x0) in H3. *)
+(*         apply map_filter_lookup_Some in H3. *)
+(*         destruct H3. *)
+(*         simplify_eq /=. *)
+(*         rewrite /get_vm_page_table /get_page_tables /update_ownership_batch *)
+(*                 /update_ownership_global_batch //= in H3. *)
+(*         rewrite vlookup_insert in H3. *)
+(*         apply elem_of_union. *)
+(*         induction ps; simpl in *. *)
+(*         -- left. *)
+(*            apply (get_owned_gmap_is_owned x0.1 H1). *)
+(*            exists (x0.2). *)
+(*            split;eauto. *)
+(*         -- destruct (decide (a=x0.1)). *)
+(*            right;set_solver. *)
+(*            assert (Himp :(x0.1 ∈ sown ∨ x0.1 ∈ ((list_to_set ps):gset PID)) *)
+(*                          ->(x0.1 ∈ sown ∨ x0.1 ∈ {[a]} ∪ ((list_to_set ps):gset PID))). *)
+(*            { intros. destruct H. left;done. right; set_solver. } *)
+(*            apply Himp. *)
+(*            apply IHps;eauto. *)
+(*            rewrite lookup_insert_ne in H3;done. *)
+(*       * intros. *)
+(*         apply elem_of_union in H2. *)
+(*         destruct H2. *)
+(*         apply (get_owned_gmap_is_owned x H1) in H2;eauto. *)
+(*         destruct H2. *)
+(*         destruct H2. *)
+(*         inv_map_in. *)
+(*         exists (x,x0). *)
+(*         split;eauto. *)
+(*         apply elem_of_list_In . *)
+(*         apply elem_of_map_to_list. *)
+(*         apply map_filter_lookup_Some. *)
+(*         rewrite /get_vm_page_table /get_page_tables /update_ownership_batch *)
+(*                 /update_ownership_global_batch /=. *)
+(*         rewrite -H0 vlookup_insert. *)
+(*         destruct H1;split;eauto. *)
+(*         generalize dependent sps. *)
+(*         induction ps;simpl in *. *)
+(*         done. *)
+(*         intros. *)
+(*         destruct (decide (x=a)). *)
+(*         subst a. *)
+(*         rewrite lookup_insert. *)
+(*         rewrite /is_owned in H3. *)
+(*         destruct x0;eauto. *)
+(*         done. *)
+(*         rewrite lookup_insert_ne;eauto. *)
+(*         inv_map_in. *)
+(*         exists (x,Owned). *)
+(*         split;eauto. *)
+(*         apply elem_of_list_In . *)
+(*         apply elem_of_map_to_list. *)
+(*         apply map_filter_lookup_Some. *)
+(*         rewrite /get_vm_page_table /get_page_tables /update_ownership_batch *)
+(*                 /update_ownership_global_batch /=. *)
+(*         split;eauto. *)
+(*         rewrite -H0 vlookup_insert //=. *)
+(*         generalize dependent sps. *)
+(*         induction ps;simpl in *. *)
+(*         intros. *)
+(*         set_solver. *)
+(*         intros. *)
+(*         destruct (decide (x=a)). *)
+(*         subst a. *)
+(*         rewrite lookup_insert //. *)
+(*         rewrite lookup_insert_ne;eauto. *)
+(*         apply (IHps (list_to_set ps));eauto. *)
+(*         set_solver. *)
+(*     } *)
+(*     apply (@elem_of_list_to_map_1' VMID (gmap VMID) _ _ _ _ _ _ _ _ gmap_finmap). *)
+(*     + intros. *)
+(*       inv_map_in. *)
+(*       inversion H2. *)
+(*       do 3 f_equal. *)
+(*       clear H6 H3 H2. *)
+(*       subst x. *)
+(*       symmetry. *)
+(*       apply Hgoal. *)
+(*     + inv_map_in. *)
+(*       exists i. *)
+(*       split;[|apply in_list_of_vmids]. *)
+(*       do 4 f_equal. *)
+(*       apply Hgoal. *)
+(*   - rewrite (lookup_insert_ne _ i i0 _);eauto. *)
+(*     set (l:= (map *)
+(*                 (λ v, *)
+(*                  (v, get_pagetable_gset (update_ownership_batch σ ps Owned) v (λ pt : page_table, pt.1) is_owned)) *)
+(*                 list_of_vmids)) in *. *)
+(*     destruct (list_to_map l !! i0) eqn:Heqn. *)
+(*     + apply (elem_of_list_to_map_2 l i0 g) in Heqn. *)
+(*       apply elem_of_list_In in Heqn. *)
+(*       apply in_map_iff in Heqn. *)
+(*       inversion Heqn;clear Heqn. *)
+(*       destruct H2 as [H3 HIn];inversion H3;subst;clear H3. *)
+(*       symmetry. *)
+(*       apply elem_of_list_to_map_1'. *)
+(*       *  intros. *)
+(*          inv_map_in. *)
+(*          inversion H. *)
+(*          rewrite /get_pagetable_gset. *)
+(*          do 5 f_equal. *)
+(*          rewrite /get_vm_page_table update_ownership_batch_preserve_other_page_tables //. *)
+(*       * inv_map_in. *)
+(*         exists i0. *)
+(*         split;eauto. *)
+(*         rewrite /get_pagetable_gset. *)
+(*         do 6 f_equal. *)
+(*         rewrite /get_vm_page_table update_ownership_batch_preserve_other_page_tables //. *)
+(*     + apply (@not_elem_of_list_to_map_2 VMID (gmap VMID) _ _ _ _ _ _ _ _ gmap_finmap) in Heqn. *)
+(*       symmetry. *)
+(*       apply not_elem_of_list_to_map_1. *)
+(*       intro P. *)
+(*       apply Heqn. *)
+(*       apply elem_of_list_In. *)
+(*       apply in_map_iff. *)
+(*       apply elem_of_list_In in P. *)
+(*       apply in_map_iff in P. *)
+(*       destruct P. *)
+(*       exists x. *)
+(*       destruct H2. *)
+(*       split;eauto. *)
+(*       apply in_map_iff. *)
+(*       apply in_map_iff in H3. *)
+(*       destruct H3. *)
+(*       exists x0. *)
+(*       destruct H3. *)
+(*       split;eauto. *)
+(*       rewrite -H3 /get_pagetable_gset. *)
+(*       do 6 f_equal. *)
+(*       rewrite /get_vm_page_table update_ownership_batch_preserve_other_page_tables //. *)
+(*       destruct x. *)
+(*       simpl in H2;inversion H3. *)
+(*         by subst. *)
+(* Qed. *)
 
-Lemma update_exclusive_batch_update_pagetable_union {σ i sexcl} {sps:gset PID} (ps: list PID):
- sps = (list_to_set ps) ->
- i = (get_current_vm σ) ->
- (get_excl_gmap σ) !! i = Some (sexcl) ->
- get_excl_gmap (update_access_batch σ ps ExclusiveAccess) =
- <[i:= (sexcl ∪ sps)]>(get_excl_gmap σ).
-Proof.
-  intros.
-  rewrite /get_excl_gmap /get_pagetable_gmap.
-  apply (@map_eq VMID (gmap VMID) _ _ _ _ _ _ _ _ gmap_finmap); eauto.
-  intro.
-  destruct(decide (i0 = i)).
-  - subst i0. rewrite lookup_insert.
-    assert(Hgoal: get_pagetable_gset (update_access_batch σ ps ExclusiveAccess) i (λ pt : page_table, pt.2) is_exclusive
-                  = sexcl ∪ sps).
-    {
-      apply set_eq.
-      intro.
-      rewrite  elem_of_list_to_set.
-      split.
-      * intros.
-        inv_map_in.
-        apply elem_of_list_In in H3.
-        apply (elem_of_map_to_list' _ x0) in H3.
-        apply map_filter_lookup_Some in H3.
-        destruct H3.
-        simplify_eq /=.
-        rewrite /get_vm_page_table /get_page_tables /update_access_batch
-                /update_access_global_batch //= in H3.
-        rewrite vlookup_insert in H3.
-        apply elem_of_union.
-        induction ps; simpl in *.
-        -- left.
-           apply (get_excl_gmap_is_exclusive_true x0.1 H1).
-           exists (x0.2).
-           split;eauto.
-        -- destruct (decide (a=x0.1)).
-           right;set_solver.
-           assert (Himp :(x0.1 ∈ sexcl ∨ x0.1 ∈ ((list_to_set ps):gset PID))
-                         ->(x0.1 ∈ sexcl ∨ x0.1 ∈ {[a]} ∪ ((list_to_set ps):gset PID))).
-           { intros. destruct H. left;done. right; set_solver. }
-           apply Himp.
-           apply IHps;eauto.
-           rewrite lookup_insert_ne in H3;done.
-      * intros.
-        apply elem_of_union in H2.
-        destruct H2.
-        apply (get_excl_gmap_is_exclusive_true x H1) in H2;eauto.
-        destruct H2.
-        destruct H2.
-        inv_map_in.
-        exists (x,x0).
-        split;eauto.
-        apply elem_of_list_In .
-        apply elem_of_map_to_list.
-        apply map_filter_lookup_Some.
-        rewrite /get_vm_page_table /get_page_tables /update_access_batch
-                /update_access_global_batch /=.
-        rewrite -H0 vlookup_insert.
-        destruct H1;split;eauto.
-        generalize dependent sps.
-        induction ps;simpl in *.
-        done.
-        intros.
-        destruct (decide (x=a)).
-        subst a.
-        rewrite lookup_insert.
-        rewrite /is_exclusive in H3.
-        destruct x0;try done.
-        rewrite lookup_insert_ne;eauto.
-        inv_map_in.
-        exists (x, ExclusiveAccess).
-        split;eauto.
-        apply elem_of_list_In .
-        apply elem_of_map_to_list.
-        apply map_filter_lookup_Some.
-        rewrite /get_vm_page_table /get_page_tables /update_access_batch
-                /update_access_global_batch /=.
-        split;eauto.
-        rewrite -H0 vlookup_insert //=.
-        generalize dependent sps.
-        induction ps;simpl in *.
-        intros.
-        set_solver.
-        intros.
-        destruct (decide (x=a)).
-        subst a.
-        rewrite lookup_insert //.
-        rewrite lookup_insert_ne;eauto.
-        apply (IHps (list_to_set ps));eauto.
-        set_solver.
-    }
-    apply (@elem_of_list_to_map_1' VMID (gmap VMID) _ _ _ _ _ _ _ _ gmap_finmap).
-    + intros.
-      inv_map_in.
-      inversion H2.
-      do 3 f_equal.
-      clear H6 H3 H2.
-      subst x.
-      symmetry.
-      apply Hgoal.
-    + inv_map_in.
-      exists i.
-      split;[|apply in_list_of_vmids].
-      do 4 f_equal.
-      apply Hgoal.
-  - rewrite (lookup_insert_ne _ i i0 _);eauto.
-    set (l:= (map (λ v, (v,
-                         get_pagetable_gset (update_access_batch σ ps ExclusiveAccess) v (λ pt : page_table, pt.2) is_exclusive))
-                  list_of_vmids)) in *.
-    destruct (list_to_map l !! i0) eqn:Heqn.
-    + apply (elem_of_list_to_map_2 l i0 g) in Heqn.
-      apply elem_of_list_In in Heqn.
-      apply in_map_iff in Heqn.
-      inversion Heqn;clear Heqn.
-      destruct H2 as [H3 HIn];inversion H3;subst;clear H3.
-      symmetry.
-      apply elem_of_list_to_map_1'.
-      *  intros.
-         inv_map_in.
-         inversion H.
-         rewrite /get_pagetable_gset.
-         do 5 f_equal.
-         rewrite /get_vm_page_table update_access_batch_preserve_other_page_tables //.
-      * inv_map_in.
-        exists i0.
-        split;eauto.
-        rewrite /get_pagetable_gset.
-        do 6 f_equal.
-        rewrite /get_vm_page_table update_access_batch_preserve_other_page_tables //.
-    + apply (@not_elem_of_list_to_map_2 VMID (gmap VMID) _ _ _ _ _ _ _ _ gmap_finmap) in Heqn.
-      symmetry.
-      apply not_elem_of_list_to_map_1.
-      intro P.
-      apply Heqn.
-      apply elem_of_list_In.
-      apply in_map_iff.
-      apply elem_of_list_In in P.
-      apply in_map_iff in P.
-      destruct P.
-      exists x.
-      destruct H2.
-      split;eauto.
-      apply in_map_iff.
-      apply in_map_iff in H3.
-      destruct H3.
-      exists x0.
-      destruct H3.
-      split;eauto.
-      rewrite -H3 /get_pagetable_gset.
-      do 6 f_equal.
-      rewrite /get_vm_page_table update_access_batch_preserve_other_page_tables //.
-      destruct x.
-      simpl in H2;inversion H3.
-        by subst.
-Qed.
+(* Lemma update_exclusive_batch_update_pagetable_union {σ i sexcl} {sps:gset PID} (ps: list PID): *)
+(*  sps = (list_to_set ps) -> *)
+(*  i = (get_current_vm σ) -> *)
+(*  (get_excl_gmap σ) !! i = Some (sexcl) -> *)
+(*  get_excl_gmap (update_access_batch σ ps ExclusiveAccess) = *)
+(*  <[i:= (sexcl ∪ sps)]>(get_excl_gmap σ). *)
+(* Proof. *)
+(*   intros. *)
+(*   rewrite /get_excl_gmap /get_pagetable_gmap. *)
+(*   apply (@map_eq VMID (gmap VMID) _ _ _ _ _ _ _ _ gmap_finmap); eauto. *)
+(*   intro. *)
+(*   destruct(decide (i0 = i)). *)
+(*   - subst i0. rewrite lookup_insert. *)
+(*     assert(Hgoal: get_pagetable_gset (update_access_batch σ ps ExclusiveAccess) i (λ pt : page_table, pt.2) is_exclusive *)
+(*                   = sexcl ∪ sps). *)
+(*     { *)
+(*       apply set_eq. *)
+(*       intro. *)
+(*       rewrite  elem_of_list_to_set. *)
+(*       split. *)
+(*       * intros. *)
+(*         inv_map_in. *)
+(*         apply elem_of_list_In in H3. *)
+(*         apply (elem_of_map_to_list' _ x0) in H3. *)
+(*         apply map_filter_lookup_Some in H3. *)
+(*         destruct H3. *)
+(*         simplify_eq /=. *)
+(*         rewrite /get_vm_page_table /get_page_tables /update_access_batch *)
+(*                 /update_access_global_batch //= in H3. *)
+(*         rewrite vlookup_insert in H3. *)
+(*         apply elem_of_union. *)
+(*         induction ps; simpl in *. *)
+(*         -- left. *)
+(*            apply (get_excl_gmap_is_exclusive_true x0.1 H1). *)
+(*            exists (x0.2). *)
+(*            split;eauto. *)
+(*         -- destruct (decide (a=x0.1)). *)
+(*            right;set_solver. *)
+(*            assert (Himp :(x0.1 ∈ sexcl ∨ x0.1 ∈ ((list_to_set ps):gset PID)) *)
+(*                          ->(x0.1 ∈ sexcl ∨ x0.1 ∈ {[a]} ∪ ((list_to_set ps):gset PID))). *)
+(*            { intros. destruct H. left;done. right; set_solver. } *)
+(*            apply Himp. *)
+(*            apply IHps;eauto. *)
+(*            rewrite lookup_insert_ne in H3;done. *)
+(*       * intros. *)
+(*         apply elem_of_union in H2. *)
+(*         destruct H2. *)
+(*         apply (get_excl_gmap_is_exclusive_true x H1) in H2;eauto. *)
+(*         destruct H2. *)
+(*         destruct H2. *)
+(*         inv_map_in. *)
+(*         exists (x,x0). *)
+(*         split;eauto. *)
+(*         apply elem_of_list_In . *)
+(*         apply elem_of_map_to_list. *)
+(*         apply map_filter_lookup_Some. *)
+(*         rewrite /get_vm_page_table /get_page_tables /update_access_batch *)
+(*                 /update_access_global_batch /=. *)
+(*         rewrite -H0 vlookup_insert. *)
+(*         destruct H1;split;eauto. *)
+(*         generalize dependent sps. *)
+(*         induction ps;simpl in *. *)
+(*         done. *)
+(*         intros. *)
+(*         destruct (decide (x=a)). *)
+(*         subst a. *)
+(*         rewrite lookup_insert. *)
+(*         rewrite /is_exclusive in H3. *)
+(*         destruct x0;try done. *)
+(*         rewrite lookup_insert_ne;eauto. *)
+(*         inv_map_in. *)
+(*         exists (x, ExclusiveAccess). *)
+(*         split;eauto. *)
+(*         apply elem_of_list_In . *)
+(*         apply elem_of_map_to_list. *)
+(*         apply map_filter_lookup_Some. *)
+(*         rewrite /get_vm_page_table /get_page_tables /update_access_batch *)
+(*                 /update_access_global_batch /=. *)
+(*         split;eauto. *)
+(*         rewrite -H0 vlookup_insert //=. *)
+(*         generalize dependent sps. *)
+(*         induction ps;simpl in *. *)
+(*         intros. *)
+(*         set_solver. *)
+(*         intros. *)
+(*         destruct (decide (x=a)). *)
+(*         subst a. *)
+(*         rewrite lookup_insert //. *)
+(*         rewrite lookup_insert_ne;eauto. *)
+(*         apply (IHps (list_to_set ps));eauto. *)
+(*         set_solver. *)
+(*     } *)
+(*     apply (@elem_of_list_to_map_1' VMID (gmap VMID) _ _ _ _ _ _ _ _ gmap_finmap). *)
+(*     + intros. *)
+(*       inv_map_in. *)
+(*       inversion H2. *)
+(*       do 3 f_equal. *)
+(*       clear H6 H3 H2. *)
+(*       subst x. *)
+(*       symmetry. *)
+(*       apply Hgoal. *)
+(*     + inv_map_in. *)
+(*       exists i. *)
+(*       split;[|apply in_list_of_vmids]. *)
+(*       do 4 f_equal. *)
+(*       apply Hgoal. *)
+(*   - rewrite (lookup_insert_ne _ i i0 _);eauto. *)
+(*     set (l:= (map (λ v, (v, *)
+(*                          get_pagetable_gset (update_access_batch σ ps ExclusiveAccess) v (λ pt : page_table, pt.2) is_exclusive)) *)
+(*                   list_of_vmids)) in *. *)
+(*     destruct (list_to_map l !! i0) eqn:Heqn. *)
+(*     + apply (elem_of_list_to_map_2 l i0 g) in Heqn. *)
+(*       apply elem_of_list_In in Heqn. *)
+(*       apply in_map_iff in Heqn. *)
+(*       inversion Heqn;clear Heqn. *)
+(*       destruct H2 as [H3 HIn];inversion H3;subst;clear H3. *)
+(*       symmetry. *)
+(*       apply elem_of_list_to_map_1'. *)
+(*       *  intros. *)
+(*          inv_map_in. *)
+(*          inversion H. *)
+(*          rewrite /get_pagetable_gset. *)
+(*          do 5 f_equal. *)
+(*          rewrite /get_vm_page_table update_access_batch_preserve_other_page_tables //. *)
+(*       * inv_map_in. *)
+(*         exists i0. *)
+(*         split;eauto. *)
+(*         rewrite /get_pagetable_gset. *)
+(*         do 6 f_equal. *)
+(*         rewrite /get_vm_page_table update_access_batch_preserve_other_page_tables //. *)
+(*     + apply (@not_elem_of_list_to_map_2 VMID (gmap VMID) _ _ _ _ _ _ _ _ gmap_finmap) in Heqn. *)
+(*       symmetry. *)
+(*       apply not_elem_of_list_to_map_1. *)
+(*       intro P. *)
+(*       apply Heqn. *)
+(*       apply elem_of_list_In. *)
+(*       apply in_map_iff. *)
+(*       apply elem_of_list_In in P. *)
+(*       apply in_map_iff in P. *)
+(*       destruct P. *)
+(*       exists x. *)
+(*       destruct H2. *)
+(*       split;eauto. *)
+(*       apply in_map_iff. *)
+(*       apply in_map_iff in H3. *)
+(*       destruct H3. *)
+(*       exists x0. *)
+(*       destruct H3. *)
+(*       split;eauto. *)
+(*       rewrite -H3 /get_pagetable_gset. *)
+(*       do 6 f_equal. *)
+(*       rewrite /get_vm_page_table update_access_batch_preserve_other_page_tables //. *)
+(*       destruct x. *)
+(*       simpl in H2;inversion H3. *)
+(*         by subst. *)
+(* Qed. *)
 
-Lemma update_access_batch_update_pagetable_union {σ i sacc a'} {sps:gset PID} (ps: list PID):
- sps = (list_to_set ps) ->
- i = (get_current_vm σ) ->
- (get_access_gmap σ) !! i = Some (sacc) ->
- sps ## sacc ->
- is_accessible a' = true ->
- get_access_gmap (update_access_batch σ ps a') =
- <[i:= (sacc ∪ sps)]>(get_access_gmap σ).
-Proof.
-  intros H H0 H1 P Q.
-  rewrite /get_access_gmap /get_pagetable_gmap.
-  apply (@map_eq VMID (gmap VMID) _ _ _ _ _ _ _ _ gmap_finmap); eauto.
-  intro.
-  destruct(decide (i0 = i)).
-  - subst i0. rewrite lookup_insert.
-    assert(Hgoal: get_pagetable_gset (update_access_batch σ ps a') i (λ pt : page_table, pt.2) is_accessible
-                  = sacc ∪ sps).
-    {
-      apply set_eq.
-      intro.
-      rewrite elem_of_list_to_set.
-      split.
-      * intros.
-        inv_map_in.
-        apply elem_of_list_In in H3.
-        apply (elem_of_map_to_list' _ x0) in H3.
-        apply map_filter_lookup_Some in H3.
-        destruct H3.
-        simplify_eq /=.
-        rewrite /get_vm_page_table /get_page_tables /update_access_batch
-                /update_access_global_batch //= in H3.
-        rewrite vlookup_insert in H3.
-        apply elem_of_union.
-        induction ps; simpl in *.
-        -- left.
-           apply (get_access_gmap_is_accessible x0.1 H1).
-           exists (x0.2).
-           split;eauto.
-        -- destruct (decide (a=x0.1)).
-           right;set_solver.
-           assert (Himp :(x0.1 ∈ sacc ∨ x0.1 ∈ ((list_to_set ps):gset PID))
-                         ->(x0.1 ∈ sacc ∨ x0.1 ∈ {[a]} ∪ ((list_to_set ps):gset PID))).
-           { intros. destruct H. left;done. right; set_solver. }
-           apply Himp.
-           apply IHps;eauto.
-           rewrite ->disjoint_union_l in P.
-           destruct P; done.
-           rewrite lookup_insert_ne in H3;done.
-      * intros.
-        apply elem_of_union in H2.
-        destruct H2.
-        pose proof H2 as H2'.
-        apply (get_access_gmap_is_accessible x H1) in H2;eauto.
-        destruct H2.
-        destruct H2.
-        inv_map_in.
-        exists (x,x0).
-        split;eauto.
-        apply elem_of_list_In .
-        apply elem_of_map_to_list.
-        apply map_filter_lookup_Some.
-        rewrite /get_vm_page_table /get_page_tables /update_access_batch
-                /update_access_global_batch /=.
-        rewrite -H0 vlookup_insert.
-        destruct H1;split;eauto.
-        simpl.
-        generalize dependent sps.
-        induction ps;simpl in *.
-        done.
-        intros.
-        destruct (decide (x=a)).
-        subst a.
-        rewrite lookup_insert.
-        rewrite /is_accessible in H3.
-        destruct x0;try done.
-        rewrite ->elem_of_disjoint in P.
-        exfalso.
-        apply P with x; set_solver.
-        rewrite ->elem_of_disjoint in P.
-        exfalso.
-        apply P with x; set_solver.
-        rewrite lookup_insert_ne; eauto.
-        apply IHps with (list_to_set ps); auto.
-        apply disjoint_union_l with {[a]}.
-        rewrite H in P; auto.
-        inv_map_in.
-        exists (x, a').
-        split;eauto.
-        apply elem_of_list_In .
-        apply elem_of_map_to_list.
-        apply map_filter_lookup_Some.
-        rewrite /get_vm_page_table /get_page_tables /update_access_batch
-                /update_access_global_batch /=.
-        split;eauto.
-        rewrite -H0 vlookup_insert //=.
-        generalize dependent sps.
-        induction ps;simpl in *.
-        intros.
-        set_solver.
-        intros.
-        destruct (decide (x=a)).
-        subst a.
-        rewrite lookup_insert //.
-        rewrite lookup_insert_ne;eauto.
-        apply (IHps (list_to_set ps));eauto.
-        set_solver.
-        set_solver.
-    }
-    apply (@elem_of_list_to_map_1' VMID (gmap VMID) _ _ _ _ _ _ _ _ gmap_finmap).
-    + intros.
-      inv_map_in.
-      inversion H2.
-      do 3 f_equal.
-      clear H6 H3 H2.
-      subst x.
-      symmetry.
-      apply Hgoal.
-    + inv_map_in.
-      exists i.
-      split;[|apply in_list_of_vmids].
-      do 4 f_equal.
-      apply Hgoal.
-  - rewrite (lookup_insert_ne _ i i0 _);eauto.
-    set (l:= (map (λ v,
-                   (v, get_pagetable_gset (update_access_batch σ ps a') v (λ pt : page_table, pt.2) is_accessible))
-                  list_of_vmids)) in *.
-    destruct (list_to_map l !! i0) eqn:Heqn.
-    + apply (elem_of_list_to_map_2 l i0 g) in Heqn.
-      apply elem_of_list_In in Heqn.
-      apply in_map_iff in Heqn.
-      inversion Heqn;clear Heqn.
-      destruct H2 as [H3 HIn];inversion H3;subst;clear H3.
-      symmetry.
-      apply elem_of_list_to_map_1'.
-      *  intros.
-         inv_map_in.
-         inversion H.
-         rewrite /get_pagetable_gset.
-         do 5 f_equal.
-         rewrite /get_vm_page_table update_access_batch_preserve_other_page_tables //.
-      * inv_map_in.
-        exists i0.
-        split;eauto.
-        rewrite /get_pagetable_gset.
-        do 6 f_equal.
-        rewrite /get_vm_page_table update_access_batch_preserve_other_page_tables //.
-    + apply (@not_elem_of_list_to_map_2 VMID (gmap VMID) _ _ _ _ _ _ _ _ gmap_finmap) in Heqn.
-      symmetry.
-      apply not_elem_of_list_to_map_1.
-      intro R.
-      apply Heqn.
-      apply elem_of_list_In.
-      apply in_map_iff.
-      apply elem_of_list_In in R.
-      apply in_map_iff in R.
-      destruct R.
-      exists x.
-      destruct H2.
-      split;eauto.
-      apply in_map_iff.
-      apply in_map_iff in H3.
-      destruct H3.
-      exists x0.
-      destruct H3.
-      split;eauto.
-      rewrite -H3 /get_pagetable_gset.
-      do 6 f_equal.
-      rewrite /get_vm_page_table update_access_batch_preserve_other_page_tables //.
-      destruct x.
-      simpl in H2;inversion H3.
-        by subst.
-Qed.
+(* Lemma update_access_batch_update_pagetable_union {σ i sacc a'} {sps:gset PID} (ps: list PID): *)
+(*  sps = (list_to_set ps) -> *)
+(*  i = (get_current_vm σ) -> *)
+(*  (get_access_gmap σ) !! i = Some (sacc) -> *)
+(*  sps ## sacc -> *)
+(*  is_accessible a' = true -> *)
+(*  get_access_gmap (update_access_batch σ ps a') = *)
+(*  <[i:= (sacc ∪ sps)]>(get_access_gmap σ). *)
+(* Proof. *)
+(*   intros H H0 H1 P Q. *)
+(*   rewrite /get_access_gmap /get_pagetable_gmap. *)
+(*   apply (@map_eq VMID (gmap VMID) _ _ _ _ _ _ _ _ gmap_finmap); eauto. *)
+(*   intro. *)
+(*   destruct(decide (i0 = i)). *)
+(*   - subst i0. rewrite lookup_insert. *)
+(*     assert(Hgoal: get_pagetable_gset (update_access_batch σ ps a') i (λ pt : page_table, pt.2) is_accessible *)
+(*                   = sacc ∪ sps). *)
+(*     { *)
+(*       apply set_eq. *)
+(*       intro. *)
+(*       rewrite elem_of_list_to_set. *)
+(*       split. *)
+(*       * intros. *)
+(*         inv_map_in. *)
+(*         apply elem_of_list_In in H3. *)
+(*         apply (elem_of_map_to_list' _ x0) in H3. *)
+(*         apply map_filter_lookup_Some in H3. *)
+(*         destruct H3. *)
+(*         simplify_eq /=. *)
+(*         rewrite /get_vm_page_table /get_page_tables /update_access_batch *)
+(*                 /update_access_global_batch //= in H3. *)
+(*         rewrite vlookup_insert in H3. *)
+(*         apply elem_of_union. *)
+(*         induction ps; simpl in *. *)
+(*         -- left. *)
+(*            apply (get_access_gmap_is_accessible x0.1 H1). *)
+(*            exists (x0.2). *)
+(*            split;eauto. *)
+(*         -- destruct (decide (a=x0.1)). *)
+(*            right;set_solver. *)
+(*            assert (Himp :(x0.1 ∈ sacc ∨ x0.1 ∈ ((list_to_set ps):gset PID)) *)
+(*                          ->(x0.1 ∈ sacc ∨ x0.1 ∈ {[a]} ∪ ((list_to_set ps):gset PID))). *)
+(*            { intros. destruct H. left;done. right; set_solver. } *)
+(*            apply Himp. *)
+(*            apply IHps;eauto. *)
+(*            rewrite ->disjoint_union_l in P. *)
+(*            destruct P; done. *)
+(*            rewrite lookup_insert_ne in H3;done. *)
+(*       * intros. *)
+(*         apply elem_of_union in H2. *)
+(*         destruct H2. *)
+(*         pose proof H2 as H2'. *)
+(*         apply (get_access_gmap_is_accessible x H1) in H2;eauto. *)
+(*         destruct H2. *)
+(*         destruct H2. *)
+(*         inv_map_in. *)
+(*         exists (x,x0). *)
+(*         split;eauto. *)
+(*         apply elem_of_list_In . *)
+(*         apply elem_of_map_to_list. *)
+(*         apply map_filter_lookup_Some. *)
+(*         rewrite /get_vm_page_table /get_page_tables /update_access_batch *)
+(*                 /update_access_global_batch /=. *)
+(*         rewrite -H0 vlookup_insert. *)
+(*         destruct H1;split;eauto. *)
+(*         simpl. *)
+(*         generalize dependent sps. *)
+(*         induction ps;simpl in *. *)
+(*         done. *)
+(*         intros. *)
+(*         destruct (decide (x=a)). *)
+(*         subst a. *)
+(*         rewrite lookup_insert. *)
+(*         rewrite /is_accessible in H3. *)
+(*         destruct x0;try done. *)
+(*         rewrite ->elem_of_disjoint in P. *)
+(*         exfalso. *)
+(*         apply P with x; set_solver. *)
+(*         rewrite ->elem_of_disjoint in P. *)
+(*         exfalso. *)
+(*         apply P with x; set_solver. *)
+(*         rewrite lookup_insert_ne; eauto. *)
+(*         apply IHps with (list_to_set ps); auto. *)
+(*         apply disjoint_union_l with {[a]}. *)
+(*         rewrite H in P; auto. *)
+(*         inv_map_in. *)
+(*         exists (x, a'). *)
+(*         split;eauto. *)
+(*         apply elem_of_list_In . *)
+(*         apply elem_of_map_to_list. *)
+(*         apply map_filter_lookup_Some. *)
+(*         rewrite /get_vm_page_table /get_page_tables /update_access_batch *)
+(*                 /update_access_global_batch /=. *)
+(*         split;eauto. *)
+(*         rewrite -H0 vlookup_insert //=. *)
+(*         generalize dependent sps. *)
+(*         induction ps;simpl in *. *)
+(*         intros. *)
+(*         set_solver. *)
+(*         intros. *)
+(*         destruct (decide (x=a)). *)
+(*         subst a. *)
+(*         rewrite lookup_insert //. *)
+(*         rewrite lookup_insert_ne;eauto. *)
+(*         apply (IHps (list_to_set ps));eauto. *)
+(*         set_solver. *)
+(*         set_solver. *)
+(*     } *)
+(*     apply (@elem_of_list_to_map_1' VMID (gmap VMID) _ _ _ _ _ _ _ _ gmap_finmap). *)
+(*     + intros. *)
+(*       inv_map_in. *)
+(*       inversion H2. *)
+(*       do 3 f_equal. *)
+(*       clear H6 H3 H2. *)
+(*       subst x. *)
+(*       symmetry. *)
+(*       apply Hgoal. *)
+(*     + inv_map_in. *)
+(*       exists i. *)
+(*       split;[|apply in_list_of_vmids]. *)
+(*       do 4 f_equal. *)
+(*       apply Hgoal. *)
+(*   - rewrite (lookup_insert_ne _ i i0 _);eauto. *)
+(*     set (l:= (map (λ v, *)
+(*                    (v, get_pagetable_gset (update_access_batch σ ps a') v (λ pt : page_table, pt.2) is_accessible)) *)
+(*                   list_of_vmids)) in *. *)
+(*     destruct (list_to_map l !! i0) eqn:Heqn. *)
+(*     + apply (elem_of_list_to_map_2 l i0 g) in Heqn. *)
+(*       apply elem_of_list_In in Heqn. *)
+(*       apply in_map_iff in Heqn. *)
+(*       inversion Heqn;clear Heqn. *)
+(*       destruct H2 as [H3 HIn];inversion H3;subst;clear H3. *)
+(*       symmetry. *)
+(*       apply elem_of_list_to_map_1'. *)
+(*       *  intros. *)
+(*          inv_map_in. *)
+(*          inversion H. *)
+(*          rewrite /get_pagetable_gset. *)
+(*          do 5 f_equal. *)
+(*          rewrite /get_vm_page_table update_access_batch_preserve_other_page_tables //. *)
+(*       * inv_map_in. *)
+(*         exists i0. *)
+(*         split;eauto. *)
+(*         rewrite /get_pagetable_gset. *)
+(*         do 6 f_equal. *)
+(*         rewrite /get_vm_page_table update_access_batch_preserve_other_page_tables //. *)
+(*     + apply (@not_elem_of_list_to_map_2 VMID (gmap VMID) _ _ _ _ _ _ _ _ gmap_finmap) in Heqn. *)
+(*       symmetry. *)
+(*       apply not_elem_of_list_to_map_1. *)
+(*       intro R. *)
+(*       apply Heqn. *)
+(*       apply elem_of_list_In. *)
+(*       apply in_map_iff. *)
+(*       apply elem_of_list_In in R. *)
+(*       apply in_map_iff in R. *)
+(*       destruct R. *)
+(*       exists x. *)
+(*       destruct H2. *)
+(*       split;eauto. *)
+(*       apply in_map_iff. *)
+(*       apply in_map_iff in H3. *)
+(*       destruct H3. *)
+(*       exists x0. *)
+(*       destruct H3. *)
+(*       split;eauto. *)
+(*       rewrite -H3 /get_pagetable_gset. *)
+(*       do 6 f_equal. *)
+(*       rewrite /get_vm_page_table update_access_batch_preserve_other_page_tables //. *)
+(*       destruct x. *)
+(*       simpl in H2;inversion H3. *)
+(*         by subst. *)
+(* Qed. *)
 
-Lemma update_access_batch_update_pagetable_idempotent {σ i sacc a'} {sps:gset PID} (ps: list PID):
- sps = (list_to_set ps) ->
- i = (get_current_vm σ) ->
- (get_access_gmap σ) !! i = Some (sacc) ->
- sps ⊆ sacc ->
- is_accessible a' = true ->
- get_access_gmap (update_access_batch σ ps a') =
- (get_access_gmap σ).
-Proof.
-  intros H H0 H1 P Q.
-  rewrite /get_access_gmap /get_pagetable_gmap.
-  apply (@map_eq VMID (gmap VMID) _ _ _ _ _ _ _ _ gmap_finmap); eauto.
-  rewrite /get_access_gmap /get_pagetable_gmap in H1.
-  intro.
-  destruct(decide (i0 = i)).
-  - subst i0.
-    rewrite H1.  
-    assert(Hgoal: get_pagetable_gset (update_access_batch σ ps a') i (λ pt : page_table, pt.2) is_accessible
-                  = sacc).
-    {
-      apply set_eq.
-      intro.
-      rewrite elem_of_list_to_set.
-      split.
-      * intros.
-        inv_map_in.
-        apply elem_of_list_In in H3.
-        apply (elem_of_map_to_list' _ x0) in H3.
-        apply map_filter_lookup_Some in H3.
-        destruct H3.
-        simplify_eq /=.
-        rewrite /get_vm_page_table /get_page_tables /update_access_batch
-                /update_access_global_batch //= in H3.
-        rewrite vlookup_insert in H3.
-        induction ps; simpl in *.
-        -- apply (get_access_gmap_is_accessible x0.1 H1).
-           exists (x0.2).
-           split;eauto.
-        -- destruct (decide (a=x0.1)).
-           set_solver.
-           apply IHps;eauto.
-           set_solver.
-           rewrite lookup_insert_ne in H3;done.
-      * intros.
-        apply (get_access_gmap_is_accessible x H1) in H2;eauto.
-        destruct H2.
-        destruct H2.
-        destruct (decide (x0=a')).
-        -- subst x0.
-           inv_map_in.
-           exists (x,a').
-           split;eauto.
-           apply elem_of_list_In .
-           apply elem_of_map_to_list.
-           apply map_filter_lookup_Some.
-           rewrite /get_vm_page_table /get_page_tables /update_access_batch
-                   /update_access_global_batch /=.
-           rewrite -H0 vlookup_insert.
-           destruct H1;split;eauto.
-           simpl.
-           generalize dependent sps.
-           induction ps;simpl in *.
-           done.
-           intros.
-           destruct (decide (x=a)).
-           subst a.
-           rewrite lookup_insert.
-           reflexivity.
-           rewrite lookup_insert_ne; eauto.
-           apply IHps with (list_to_set ps); auto.
-           rewrite H in P.
-           rewrite ->union_subseteq in P.
-           destruct P; auto.
-        -- inv_map_in.
-           destruct (decide (x ∈ ps)).
-           ++ exists (x, a').
-              split; auto.
-              apply elem_of_list_In.
-              apply elem_of_map_to_list'.
-              apply map_filter_lookup_Some.
-              split; auto.
-              simpl.
-              rewrite /update_access_batch /update_access_global_batch /get_vm_page_table /get_page_tables.
-              simpl.
-              rewrite H0.
-              rewrite <-H0.
-              rewrite /get_vm_page_table /get_page_tables in H2.
-              rewrite vlookup_insert.
-              simpl.
-              generalize dependent sps.
-              induction ps;simpl in *.
-              set_solver.
-              intros.
-              destruct (decide (a = x)).
-              - subst a.
-                apply lookup_insert.
-              - rewrite lookup_insert_ne; auto.
-                apply IHps with (list_to_set ps); auto.
-                set_solver.
-                rewrite H in P.
-                rewrite ->union_subseteq in P.
-                destruct P; auto.
-           ++ exists (x, x0).
-              split; auto.
-              apply elem_of_list_In.
-              apply elem_of_map_to_list'.
-              apply map_filter_lookup_Some.
-              split; auto.
-              simpl.
-              rewrite /update_access_batch /update_access_global_batch /get_vm_page_table /get_page_tables.
-              simpl.
-              rewrite H0.
-              rewrite <-H0.
-              rewrite /get_vm_page_table /get_page_tables in H2.
-              rewrite vlookup_insert.
-              simpl.
-              generalize dependent sps.
-              induction ps;simpl in *.
-              set_solver.
-              intros.
-              destruct (decide (a = x)).
-              - subst a.
-                set_solver.
-              - rewrite lookup_insert_ne; auto.
-                apply IHps with (list_to_set ps); auto.
-                set_solver.
-                rewrite H in P.
-                rewrite ->union_subseteq in P.
-                destruct P; auto.
-    }
-    apply (@elem_of_list_to_map_1' VMID (gmap VMID) _ _ _ _ _ _ _ _ gmap_finmap).
-    + intros.
-      inv_map_in.
-      inversion H2.
-      subst x.
-      symmetry.
-      apply Hgoal.
-    + inv_map_in.
-      exists i.
-      split;[|apply in_list_of_vmids].
-      do 4 f_equal.
-      apply Hgoal.
-  - set (l:= (map (λ v,
-                   (v, get_pagetable_gset (update_access_batch σ ps a') v (λ pt : page_table, pt.2) is_accessible))
-                  list_of_vmids)) in *.
-    destruct (list_to_map l !! i0) eqn:Heqn.
-    + apply (elem_of_list_to_map_2 l i0 g) in Heqn.
-      apply elem_of_list_In in Heqn.
-      apply in_map_iff in Heqn.
-      inversion Heqn;clear Heqn.
-      destruct H2 as [H3 HIn];inversion H3;subst;clear H3.
-      symmetry.
-      apply elem_of_list_to_map_1'.
-      *  intros.
-         inv_map_in.
-         inversion H.
-         rewrite /get_pagetable_gset.
-         do 5 f_equal.
-         rewrite /get_vm_page_table update_access_batch_preserve_other_page_tables //.
-      * inv_map_in.
-        exists i0.
-        split;eauto.
-        rewrite /get_pagetable_gset.
-        do 6 f_equal.
-        rewrite /get_vm_page_table update_access_batch_preserve_other_page_tables //.
-    + apply (@not_elem_of_list_to_map_2 VMID (gmap VMID) _ _ _ _ _ _ _ _ gmap_finmap) in Heqn.
-      symmetry.
-      apply not_elem_of_list_to_map_1.
-      intro R.
-      apply Heqn.
-      apply elem_of_list_In.
-      apply in_map_iff.
-      apply elem_of_list_In in R.
-      apply in_map_iff in R.
-      destruct R.
-      exists x.
-      destruct H2.
-      split;eauto.
-      apply in_map_iff.
-      apply in_map_iff in H3.
-      destruct H3.
-      exists x0.
-      destruct H3.
-      split;eauto.
-      rewrite -H3 /get_pagetable_gset.
-      do 6 f_equal.
-      rewrite /get_vm_page_table update_access_batch_preserve_other_page_tables //.
-      destruct x.
-      simpl in H2;inversion H3.
-        by subst.
-Qed.
+(* Lemma update_access_batch_update_pagetable_idempotent {σ i sacc a'} {sps:gset PID} (ps: list PID): *)
+(*  sps = (list_to_set ps) -> *)
+(*  i = (get_current_vm σ) -> *)
+(*  (get_access_gmap σ) !! i = Some (sacc) -> *)
+(*  sps ⊆ sacc -> *)
+(*  is_accessible a' = true -> *)
+(*  get_access_gmap (update_access_batch σ ps a') = *)
+(*  (get_access_gmap σ). *)
+(* Proof. *)
+(*   intros H H0 H1 P Q. *)
+(*   rewrite /get_access_gmap /get_pagetable_gmap. *)
+(*   apply (@map_eq VMID (gmap VMID) _ _ _ _ _ _ _ _ gmap_finmap); eauto. *)
+(*   rewrite /get_access_gmap /get_pagetable_gmap in H1. *)
+(*   intro. *)
+(*   destruct(decide (i0 = i)). *)
+(*   - subst i0. *)
+(*     rewrite H1.   *)
+(*     assert(Hgoal: get_pagetable_gset (update_access_batch σ ps a') i (λ pt : page_table, pt.2) is_accessible *)
+(*                   = sacc). *)
+(*     { *)
+(*       apply set_eq. *)
+(*       intro. *)
+(*       rewrite elem_of_list_to_set. *)
+(*       split. *)
+(*       * intros. *)
+(*         inv_map_in. *)
+(*         apply elem_of_list_In in H3. *)
+(*         apply (elem_of_map_to_list' _ x0) in H3. *)
+(*         apply map_filter_lookup_Some in H3. *)
+(*         destruct H3. *)
+(*         simplify_eq /=. *)
+(*         rewrite /get_vm_page_table /get_page_tables /update_access_batch *)
+(*                 /update_access_global_batch //= in H3. *)
+(*         rewrite vlookup_insert in H3. *)
+(*         induction ps; simpl in *. *)
+(*         -- apply (get_access_gmap_is_accessible x0.1 H1). *)
+(*            exists (x0.2). *)
+(*            split;eauto. *)
+(*         -- destruct (decide (a=x0.1)). *)
+(*            set_solver. *)
+(*            apply IHps;eauto. *)
+(*            set_solver. *)
+(*            rewrite lookup_insert_ne in H3;done. *)
+(*       * intros. *)
+(*         apply (get_access_gmap_is_accessible x H1) in H2;eauto. *)
+(*         destruct H2. *)
+(*         destruct H2. *)
+(*         destruct (decide (x0=a')). *)
+(*         -- subst x0. *)
+(*            inv_map_in. *)
+(*            exists (x,a'). *)
+(*            split;eauto. *)
+(*            apply elem_of_list_In . *)
+(*            apply elem_of_map_to_list. *)
+(*            apply map_filter_lookup_Some. *)
+(*            rewrite /get_vm_page_table /get_page_tables /update_access_batch *)
+(*                    /update_access_global_batch /=. *)
+(*            rewrite -H0 vlookup_insert. *)
+(*            destruct H1;split;eauto. *)
+(*            simpl. *)
+(*            generalize dependent sps. *)
+(*            induction ps;simpl in *. *)
+(*            done. *)
+(*            intros. *)
+(*            destruct (decide (x=a)). *)
+(*            subst a. *)
+(*            rewrite lookup_insert. *)
+(*            reflexivity. *)
+(*            rewrite lookup_insert_ne; eauto. *)
+(*            apply IHps with (list_to_set ps); auto. *)
+(*            rewrite H in P. *)
+(*            rewrite ->union_subseteq in P. *)
+(*            destruct P; auto. *)
+(*         -- inv_map_in. *)
+(*            destruct (decide (x ∈ ps)). *)
+(*            ++ exists (x, a'). *)
+(*               split; auto. *)
+(*               apply elem_of_list_In. *)
+(*               apply elem_of_map_to_list'. *)
+(*               apply map_filter_lookup_Some. *)
+(*               split; auto. *)
+(*               simpl. *)
+(*               rewrite /update_access_batch /update_access_global_batch /get_vm_page_table /get_page_tables. *)
+(*               simpl. *)
+(*               rewrite H0. *)
+(*               rewrite <-H0. *)
+(*               rewrite /get_vm_page_table /get_page_tables in H2. *)
+(*               rewrite vlookup_insert. *)
+(*               simpl. *)
+(*               generalize dependent sps. *)
+(*               induction ps;simpl in *. *)
+(*               set_solver. *)
+(*               intros. *)
+(*               destruct (decide (a = x)). *)
+(*               - subst a. *)
+(*                 apply lookup_insert. *)
+(*               - rewrite lookup_insert_ne; auto. *)
+(*                 apply IHps with (list_to_set ps); auto. *)
+(*                 set_solver. *)
+(*                 rewrite H in P. *)
+(*                 rewrite ->union_subseteq in P. *)
+(*                 destruct P; auto. *)
+(*            ++ exists (x, x0). *)
+(*               split; auto. *)
+(*               apply elem_of_list_In. *)
+(*               apply elem_of_map_to_list'. *)
+(*               apply map_filter_lookup_Some. *)
+(*               split; auto. *)
+(*               simpl. *)
+(*               rewrite /update_access_batch /update_access_global_batch /get_vm_page_table /get_page_tables. *)
+(*               simpl. *)
+(*               rewrite H0. *)
+(*               rewrite <-H0. *)
+(*               rewrite /get_vm_page_table /get_page_tables in H2. *)
+(*               rewrite vlookup_insert. *)
+(*               simpl. *)
+(*               generalize dependent sps. *)
+(*               induction ps;simpl in *. *)
+(*               set_solver. *)
+(*               intros. *)
+(*               destruct (decide (a = x)). *)
+(*               - subst a. *)
+(*                 set_solver. *)
+(*               - rewrite lookup_insert_ne; auto. *)
+(*                 apply IHps with (list_to_set ps); auto. *)
+(*                 set_solver. *)
+(*                 rewrite H in P. *)
+(*                 rewrite ->union_subseteq in P. *)
+(*                 destruct P; auto. *)
+(*     } *)
+(*     apply (@elem_of_list_to_map_1' VMID (gmap VMID) _ _ _ _ _ _ _ _ gmap_finmap). *)
+(*     + intros. *)
+(*       inv_map_in. *)
+(*       inversion H2. *)
+(*       subst x. *)
+(*       symmetry. *)
+(*       apply Hgoal. *)
+(*     + inv_map_in. *)
+(*       exists i. *)
+(*       split;[|apply in_list_of_vmids]. *)
+(*       do 4 f_equal. *)
+(*       apply Hgoal. *)
+(*   - set (l:= (map (λ v, *)
+(*                    (v, get_pagetable_gset (update_access_batch σ ps a') v (λ pt : page_table, pt.2) is_accessible)) *)
+(*                   list_of_vmids)) in *. *)
+(*     destruct (list_to_map l !! i0) eqn:Heqn. *)
+(*     + apply (elem_of_list_to_map_2 l i0 g) in Heqn. *)
+(*       apply elem_of_list_In in Heqn. *)
+(*       apply in_map_iff in Heqn. *)
+(*       inversion Heqn;clear Heqn. *)
+(*       destruct H2 as [H3 HIn];inversion H3;subst;clear H3. *)
+(*       symmetry. *)
+(*       apply elem_of_list_to_map_1'. *)
+(*       *  intros. *)
+(*          inv_map_in. *)
+(*          inversion H. *)
+(*          rewrite /get_pagetable_gset. *)
+(*          do 5 f_equal. *)
+(*          rewrite /get_vm_page_table update_access_batch_preserve_other_page_tables //. *)
+(*       * inv_map_in. *)
+(*         exists i0. *)
+(*         split;eauto. *)
+(*         rewrite /get_pagetable_gset. *)
+(*         do 6 f_equal. *)
+(*         rewrite /get_vm_page_table update_access_batch_preserve_other_page_tables //. *)
+(*     + apply (@not_elem_of_list_to_map_2 VMID (gmap VMID) _ _ _ _ _ _ _ _ gmap_finmap) in Heqn. *)
+(*       symmetry. *)
+(*       apply not_elem_of_list_to_map_1. *)
+(*       intro R. *)
+(*       apply Heqn. *)
+(*       apply elem_of_list_In. *)
+(*       apply in_map_iff. *)
+(*       apply elem_of_list_In in R. *)
+(*       apply in_map_iff in R. *)
+(*       destruct R. *)
+(*       exists x. *)
+(*       destruct H2. *)
+(*       split;eauto. *)
+(*       apply in_map_iff. *)
+(*       apply in_map_iff in H3. *)
+(*       destruct H3. *)
+(*       exists x0. *)
+(*       destruct H3. *)
+(*       split;eauto. *)
+(*       rewrite -H3 /get_pagetable_gset. *)
+(*       do 6 f_equal. *)
+(*       rewrite /get_vm_page_table update_access_batch_preserve_other_page_tables //. *)
+(*       destruct x. *)
+(*       simpl in H2;inversion H3. *)
+(*         by subst. *)
+(* Qed. *)
 
 
 End pagetable_extra.
@@ -1109,9 +1136,8 @@ Ltac rewrite_ownership_all :=
     try rewrite -> update_ownership_batch_preserve_current_vm;
     try rewrite -> update_ownership_batch_preserve_regs;
     try rewrite -> update_ownership_batch_preserve_mem;
-    try rewrite -> update_ownership_batch_preserve_tx;
-    try rewrite -> update_ownership_batch_preserve_rx1;
-    try rewrite -> update_ownership_batch_preserve_rx2;
+    try rewrite -> update_ownership_batch_preserve_mb;
+    try rewrite -> update_ownership_batch_preserve_rx;
     try rewrite -> update_ownership_batch_preserve_trans;
     try rewrite -> update_ownership_batch_preserve_trans';
     try rewrite -> update_ownership_batch_preserve_hpool;
@@ -1124,9 +1150,8 @@ Ltac rewrite_access_all :=
     try rewrite -> update_access_batch_preserve_current_vm;
     try rewrite -> update_access_batch_preserve_regs;
     try rewrite -> update_access_batch_preserve_mem;
-    try rewrite -> update_access_batch_preserve_tx;
-    try rewrite -> update_access_batch_preserve_rx1;
-    try rewrite -> update_access_batch_preserve_rx2;
+    try rewrite -> update_access_batch_preserve_mb;
+    try rewrite -> update_access_batch_preserve_rx;
     try rewrite -> update_access_batch_preserve_trans;
     try rewrite -> update_access_batch_preserve_trans';
     try rewrite -> update_access_batch_preserve_hpool;
